coq-SystemRF-3.0/SystemRF/LemmasInversion.v
@@ -1,0 +1,195 @@
+Require Import SystemRF.BasicDefinitions.
+Require Import SystemRF.Names.
+Require Import SystemRF.BasicPropsSubstitution.
+Require Import SystemRF.BasicPropsEnvironments.
+Require Import SystemRF.PrimitivesFTyping.
+Require Import SystemRF.WellFormedness.
+Require Import SystemRF.BasicPropsWellFormedness.
+Require Import SystemRF.Typing.
+Require Import SystemRF.LemmasTyping.
+Require Import SystemRF.LemmasSubtyping.
+Require Import SystemRF.LemmasNarrowing.
+Require Import SystemRF.LemmasTransitive. 
+
+(* -- A collection of Lemmas about inverting typing judgements for abstraction types. In our
+   --   system this is not trivial because TSub could be used finitely many times to produce
+   --   the judgment. The key point is to use transitivity of subtyping to collapse a chain
+   --   of applications of T-Sub to a single use of T-Sub *)
+
+Lemma lem_invert_lambda : forall (g:env) (le:expr) (t:type),
+  Hastype g le t -> (forall (e : expr) (s_x s : type),
+    le = Lambda e -> WFEnv g -> Subtype g t (TFunc s_x s)
+                  -> WFtype g (TFunc s_x s) Star
+                  -> exists nms, forall (y:vname), (~ Elem y nms 
+                      -> Hastype (ECons y s_x g) (unbind y e) (unbindT y s))).
+Proof. apply ( Hastype_ind
+    ( fun (g:env) (le:expr) (t:type) => forall (e : expr) (s_x s : type),
+        le = Lambda e -> WFEnv g -> Subtype g t (TFunc s_x s) 
+                      -> WFtype g (TFunc s_x s) Star
+                      -> exists nms, forall (y:vname), (~ Elem y nms 
+                          -> Hastype (ECons y s_x g) (unbind y e) (unbindT y s)))
+  ); try discriminate; intros.
+  - (* isTAbs *) inversion H4; injection H2 as H2; subst e0;   (* invert SFunc *)
+    inversion H5; try inversion H2;                             (* invert WFFunc *)
+    exists (union (union (union nms nms0) nms1) (binds g)); intros;
+    repeat (apply not_elem_union_elim in H18; destruct H18);
+    apply TSub with (unbindT y t) k;
+    try apply lem_narrow_typ_top with t_x k_x0 k_x;
+    try apply H0; try apply H16; try apply H12; 
+    try apply wfenv_unique; try assumption.
+  - (* isTSub *)
+    apply H0; try apply lem_sub_trans with t Star k Star;
+    try (apply lem_typing_wf with e; assumption); assumption.
+  Qed.
+
+Lemma lem_invert_tabs : forall (g:env) (e:expr) (t_x t:type),
+    Hastype g (Lambda e) (TFunc t_x t) 
+                  -> WFEnv g -> WFtype g (TFunc t_x t) Star
+                  -> exists nms, forall (y:vname), (~ Elem y nms 
+                          -> Hastype (ECons y t_x g) (unbind y e) (unbindT y t)).
+Proof. intros; inversion H.
+  - (* isTAbs *) exists nms; apply H7.
+  - (* isTSub *) apply lem_invert_lambda with (Lambda e) s;
+    destruct k; try (apply H3 || (apply WFKind; apply H3)); trivial.
+  Qed.
+
+Lemma lem_invert_lambdat : forall (g:env) (lke:expr) (t:type),
+    Hastype g lke t -> ( forall (k:kind) (e:expr) (s:type),
+        lke = LambdaT k e -> WFEnv g -> Subtype g t (TPoly k s)
+                          -> WFtype g (TPoly k s) Star
+                          -> exists nms, forall (a:vname), ( ~ Elem a nms 
+                                -> Hastype (EConsT a k g) (unbind_tv a e) (unbind_tvT a s))).
+Proof. apply ( Hastype_ind
+    ( fun (g:env) (lke:expr) (t:type) => forall (k:kind) (e:expr) (s:type),
+        lke = LambdaT k e -> WFEnv g -> Subtype g t (TPoly k s)
+                          -> WFtype g (TPoly k s) Star
+                          -> exists nms, forall (a:vname), ( ~ Elem a nms 
+                               -> Hastype (EConsT a k g) (unbind_tv a e) (unbind_tvT a s)))  
+  ); try discriminate; intros.
+  - (* isTAbsT *) inversion (* of SPoly *) H3; injection H1 as H1 H1'; subst k0 e0;
+    inversion (* of WFPoly *) H4; try inversion H1;
+    exists (union (union (union nms nms0) nms1) (binds g)); intros;
+    repeat (apply not_elem_union_elim in H15; destruct H15);
+    apply TSub with (unbind_tvT a t) k_t;
+    try apply H; try apply H12; try apply H7; trivial.
+  - (* isTSub *) apply H0; try apply lem_sub_trans with t Star k Star;
+    try (apply lem_typing_wf with e; assumption); assumption.
+  Qed.
+
+Lemma lem_invert_tabst : forall (g:env) (k:kind) (e:expr) (t:type),
+    Hastype g (LambdaT k e) (TPoly k t) 
+                  -> WFEnv g -> WFtype g (TPoly k t) Star
+                  -> exists nms, forall (a:vname), (~ Elem a nms 
+                          -> Hastype (EConsT a k g) (unbind_tv a e) (unbind_tvT a t)).
+Proof. intros; inversion H.
+  - (* isTAbs *) exists nms; assumption.
+  - (* isTSub *) apply lem_invert_lambdat with (LambdaT k e) s; trivial.
+  Qed.
+
+Lemma lem_lambdaT_tpoly_same_kind' : forall (g:env) (lke:expr) (t:type),
+    Hastype g lke t -> ( forall (k k':kind) (e:expr) (s:type),
+        lke = LambdaT k e -> WFEnv g -> Subtype g t (TPoly k' s)
+                          -> WFtype g (TPoly k' s) Star
+                          -> k = k').
+Proof. apply ( Hastype_ind
+    ( fun (g:env) (lke:expr) (t:type) => forall (k k':kind) (e:expr) (s:type),
+        lke = LambdaT k e -> WFEnv g -> Subtype g t (TPoly k' s)
+                          -> WFtype g (TPoly k' s) Star
+                          -> k = k') 
+  ); try discriminate; intros.
+  - (* isTAbsT *) inversion H3; injection H1 as Hk0 He0; subst k0; assumption.
+  - (* isTSub *) apply H0 with e0 s0; try apply lem_sub_trans with t Star k Star;
+    try assumption; try apply lem_typing_wf with e; trivial. Qed.
+
+Lemma lem_lambdaT_tpoly_same_kind : forall (g:env) (k k':kind) (e:expr) (t:type),
+    Hastype g (LambdaT k e) (TPoly k' t) -> WFEnv g -> WFtype g (TPoly k' t) Star  
+                                        -> k = k'.
+Proof. intros; inversion H.
+  - (* isTAbsT *) reflexivity.
+  - (* isTSub  *) apply lem_lambdaT_tpoly_same_kind'
+       with g (LambdaT k e) s e t; trivial. Qed.
+
+Lemma lem_exact_length_type : 
+  forall (g:env) (v:expr) (t:type) (ps:preds) (k:kind),
+    isList v -> isValue v 
+      -> Hastype g v (TList t ps) -> WFtype g t k -> WFEnv g 
+      -> Hastype g v (TList t (PCons (eq (length t (BV 0)) (length t v)) ps)).
+Proof.  intros. destruct v;
+  simpl in H; try contradiction.
+  pose proof TNil. pose proof TCons.
+  apply TSub with (TList t ps) Star.
+  Focus 3. 
+  apply SList with (binds g).
+  Focus 2.
+  intros.
+
+Lemma lem_invert_cons : forall (g:env) (ce:expr) (t:type),
+  Hastype g ce t -> (forall (v1 v2 : expr) (s : type),
+    ce = Cons v1 v2 -> WFEnv g -> Subtype g t (TList s PEmpty)
+                    -> WFtype g s Star
+                    -> Hastype g v2 (TList s PEmpty)).
+Proof. apply ( Hastype_ind
+    ( fun (g:env) (ce:expr) (t:type) => forall (v1 v2 : expr) (s : type),
+        ce = Cons v1 v2 -> WFEnv g -> Subtype g t (TList s PEmpty) 
+                        -> WFtype g s Star
+                        -> Hastype g v2 (TList s PEmpty))
+  ); try discriminate; intros.
+  - (* isTCons *) injection H5 as Hv1 Hv2; subst eH eT.
+    apply lem_typing_wf in H1 as p_g_t; try apply H6.
+    apply lem_wftype_islct in p_g_t as Hlct.
+    apply TSub with 
+      (TExists (TList t ps) 
+        (TList t (PCons (eq (length t (BV 0)) 
+                          (App (Prim Succ) (length t (BV 1)))) PEmpty)))
+      Star; try apply H7.
+    pose proof SBind as HSB.
+    pose proof SWitn as HSW.
+    apply TSub with 
+      (tsubBV v2 (TList t (PCons (eq (length t (BV 0)) 
+                                    (App (Prim Succ) (length t (BV 1)))) PEmpty)))
+      Star.
+    unfold tsubBV; simpl.
+    pose proof lem_subBV_at_lc_at as [_ [Hsubt _]];
+    repeat rewrite Hsubt with t 1 v2 0 0;
+    try rewrite Hsubt with t 0 v2 0 0; auto.
+    apply TSub with (TList t ps) Star; try apply H3.
+    Focus 2.
+    apply SList with (binds g); try apply lem_sub_refl with Star;
+    try apply p_g_t; intros.
+    
+    
+  
+  
+  inversion H5; subst eH eT. 
+    inversion H7.
+    set (y := fresh nms). pose proof (fresh_not_elem nms);
+    apply (H14 y) in H15 as Hsub;
+    unfold unbindT in Hsub; simpl in Hsub. inversion Hsub.
+    apply lem_typing_wf in H1 as p_g_t;
+    try apply lem_wftype_islct in p_g_t as Hlct;
+    pose proof lem_open_at_lc_at as [_ [Hopen _]];
+    try rewrite Hopen with t 0 0 y in H20. 
+    pose proof SList.
+
+    inversion H5; try inversion H2;                             (* invert WFFunc *)
+    apply TSub with (TExists (TList t ps) (TList t (PCons (eq (length t (BV 0)) (App (Prim Succ) (length t (BV 1)))) PEmpty))) Star.
+    try apply TCons. apply TCons.
+    
+    try apply lem_narrow_typ_top with t_x k_x0 k_x;
+    try apply H0; try apply H16; try apply H12; 
+    try apply wfenv_unique; try assumption.
+  - (* isTSub *)
+    apply H0; try apply lem_sub_trans with t Star k Star;
+    try (apply lem_typing_wf with e; assumption); assumption.
+  Qed.       
+
+Lemma lem_invert_tlist : forall (g:env) (v1 v2:expr) (t:type),
+    Hastype g (Cons v1 v2) (TList t PEmpty) 
+                  -> WFEnv g -> WFtype g t Star
+                  -> isValue v1 -> isValue v2
+                  -> Hastype g v2 (TList t PEmpty).
+Proof. intros; inversion H.
+  - (* isTAbs *) exists nms; apply H7.
+  - (* isTSub *) apply lem_invert_lambda with (Lambda e) s;
+    destruct k; try (apply H3 || (apply WFKind; apply H3)); trivial.
+  Qed.       
