coq-SystemRF-3.0/SystemRF/LemmasTransitive.v
@@ -1,0 +1,278 @@
+Require Import Arith.
+
+Require Import SystemRF.BasicDefinitions.
+Require Import SystemRF.Names.
+Require Import SystemRF.BasicPropsSubstitution.
+Require Import SystemRF.BasicPropsEnvironments.
+Require Import SystemRF.WellFormedness.
+Require Import SystemRF.BasicPropsWellFormedness.
+Require Import SystemRF.Typing.
+Require Import SystemRF.LemmasWeakenWF.
+Require Import SystemRF.LemmasWellFormedness.
+Require Import SystemRF.SubstitutionLemmaWF.
+Require Import SystemRF.LemmasTyping.
+Require Import SystemRF.LemmasWeakenTyp.
+Require Import SystemRF.SubstitutionLemmaTyp.
+Require Import SystemRF.LemmasNarrowing.
+
+(* Idea: We have to prove the Transitive Subtyping Lemma by induction on 
+      the combined depth of the types involved *)
+
+Fixpoint depth (t : type) : nat :=
+    match t with
+    | (TRefn b ps)    => 0
+    | (TFunc tx t')   => 1 + max (depth tx) (depth t')
+    | (TExists tx t') => 1 + max (depth tx) (depth t')
+    | (TPoly k t')    => 1 + depth t'
+    | (TList t' ps)   => 1 + depth t'
+    end.
+
+Lemma depth_tsubBV_at : forall (j:index) (v:expr) (t:type),
+    depth (tsubBV_at j v t) = depth t.
+Proof. intros j v t; revert v; revert j; induction t; intros;
+  simpl; reflexivity || f_equal; apply IHt || f_equal;
+  try apply IHt1; try apply IHt2. Qed.
+
+Lemma depth_tsubBV : forall (v:expr) (t:type),
+    depth (tsubBV v t) = depth t.
+Proof. intros; apply depth_tsubBV_at. Qed.
+
+Lemma depth_open_tvT_at : forall (j:index) (a:vname) (t:type),
+    depth (open_tvT_at j a t) = depth t.
+Proof. intros j a t; revert j; induction t; intros;
+  simpl; try destruct b; try destruct (Nat.eqb j i); 
+  reflexivity || f_equal; apply IHt || f_equal;
+  try apply IHt1; try apply IHt2; apply H. Qed.
+
+Lemma depth_unbind_tvT : forall (a:vname) (t:type),
+    depth (unbind_tvT a t) = depth t.
+Proof. intros; apply depth_open_tvT_at; assumption. Qed.
+
+Lemma depth_unbindT : forall (y:vname) (t:type),
+    depth (unbindT y t) = depth t.
+Proof. intros; rewrite lem_unbindT_is_tsubBV; 
+  apply depth_tsubBV_at; simpl; trivial. Qed.
+
+Lemma lem_sub_trans' : forall (n:nat) (g:env) (t t' t'':type) (k k' k'':kind),
+    depth t + depth t' + depth t'' <= n
+                    -> WFEnv g -> WFtype g t k 
+                    -> WFtype g t' k' -> WFtype g t'' k'' 
+                    -> Subtype g t t' -> Subtype g t' t'' 
+                    -> Subtype g t t''.
+Proof. intros n; induction n.
+  - (* Base *) intros; assert (depth t + depth t' + depth t'' = 0) 
+      by auto with *.
+    repeat (apply Nat.eq_add_0 in H6; destruct H6);
+    destruct t;   simpl in H6; try discriminate H6;
+    destruct t';  simpl in H8; try discriminate H8;
+    destruct t''; simpl in H7; try discriminate H7;
+    inversion H4; inversion H5; subst b0; subst b1;
+    apply SBase with (union nms nms0); intros;
+    apply not_elem_union_elim in H13; destruct H13;
+    apply ITrans with (unbindP y ps0); apply H11 || apply H17; trivial.
+  - (* Inductive *) intros; inversion H4; inversion H5;
+    try (subst t'; discriminate);
+    (* -ANY- SWitn *) try ( rewrite H9 || rewrite H8;
+      apply SWitn with v_x; trivial;
+      apply IHn with t' k k' k''; try rewrite depth_tsubBV;
+      subst t''; simpl in H;
+      repeat rewrite <- plus_n_Sm in H; rewrite <- Nat.succ_le_mono in H;
+      assert (depth t'0 <= max (depth t_x) (depth t'0)) 
+        as Hdep by apply Nat.le_max_r;
+      apply Nat.add_le_mono_l with (depth t'0) (max (depth t_x) (depth t'0))
+                                  (depth t + depth t') in Hdep;
+      try apply Nat.le_trans with (depth t + depth t' + Init.Nat.max (depth t_x) 
+                                                                 (depth t'0));
+      trivial; inversion H3; 
+      try inversion H16; try inversion H15; try apply WFKind;
+      pose proof (fresh_var_not_elem (union nms nms0) g) as Hy;
+      set (y := fresh_var (union nms nms0) g) in Hy; destruct Hy as [Hy Hy'];
+      apply not_elem_union_elim in Hy; destruct Hy;  
+      try rewrite lem_tsubFV_unbindT with y v_x t'0;
+      try apply lem_subst_wf_top with t_x;
+      try apply lem_typing_hasftype;
+      pose proof (lem_free_bound_in_env g (TExists t_x t'0) k'' y H3 Hy') as Hfr;
+      simpl in Hfr; destruct Hfr as [Hfr _];
+      apply not_elem_union_elim in Hfr as [_ Hfr]; 
+      try apply wfenv_unique; simpl; intuition );
+    (* SBind -ANY- *) try ( subst t; try set (nms0 := g1); inversion H1; try inversion H9; 
+      apply SBind with (union (union nms nms1) (binds g));
+      try apply lem_wftype_islct with g k''; try (subst t''; assumption);
+      intros y Hy; apply IHn with t' k k' k'';
+      try rewrite H16; try rewrite H15; try rewrite H14;
+      try rewrite depth_unbindT; subst t; simpl in H;
+      rewrite <- Nat.succ_le_mono in H;
+      assert (depth t0 <= max (depth t_x) (depth t0)) 
+        as Hdep by apply Nat.le_max_r;
+      apply Nat.add_le_mono_r with (depth t0) (max (depth t_x) (depth t0))
+                                  (depth t' + depth t'') in Hdep;
+      repeat rewrite Nat.add_assoc in Hdep;
+      try apply Nat.le_trans with (max (depth t_x) (depth t0) + depth t' + depth t'');
+      trivial; try apply WFEBind with k_x;
+      try apply H19; try apply H20; try apply H21;
+      try (destruct k; apply H23 || (apply WFKind; apply H23)); 
+      try (destruct k; apply H24 || (apply WFKind; apply H24)); 
+      try (destruct k; apply H25 || (apply WFKind; apply H25));
+      try apply lem_weaken_wf_top;
+      try apply H7; try apply lem_weaken_subtype_top with k' k'';
+      apply not_elem_union_elim in Hy; destruct Hy as [Hy Hg];
+      apply not_elem_union_elim in Hy; destruct Hy as [Hy Hy1];
+      try apply wfenv_unique; trivial).
+    * (* SBase SBase *) subst t'; injection H12 as Hb0 Hp0;
+      subst b0; subst p0; apply SBase with (union nms nms0); 
+      intros; apply not_elem_union_elim in H9; destruct H9;
+      apply ITrans with (unbindP y p2); apply H6 || apply H10; trivial.
+    * (* SFunc SFunc *) 
+      subst t; subst t'; subst t''; inversion H1; try inversion H9;
+      subst k; subst g1; subst t_x; subst t;
+      inversion H2; try inversion H9;
+      subst k'; subst g1; subst t_x; subst t;
+      inversion H3; try inversion H9;
+      subst k''; subst g1; subst t_x; subst t;  
+      simpl in H; rewrite <- Nat.succ_le_mono in H;
+      injection H14 as Hs2 Ht2; subst s0; subst t0;
+      apply SFunc with (union (union (union (union (union nms nms0) 
+                                                    nms1) nms2) nms3) (binds g));
+      assert (Subtype g s3 s1) as p_s3_s1
+      (* s3 <: s2 <: s1 *) by (apply IHn with s2 k_x1 k_x0 k_x;
+        try rewrite Nat.add_comm; try rewrite (Nat.add_comm (depth s3) (depth s2));
+        try rewrite Nat.add_assoc;
+        assert (depth s1 <= max (depth s1) (depth t1)) 
+          as Hdep1 by apply Nat.le_max_l;
+        assert (depth s2 <= max (depth s2) (depth t2)) 
+          as Hdep2 by apply Nat.le_max_l;
+        assert (depth s3 <= max (depth s3) (depth t3)) 
+          as Hdep3 by apply Nat.le_max_l;
+        repeat rewrite <- plus_n_Sm in H; simpl in H; 
+        apply Nat.lt_le_incl in H; apply Nat.lt_le_incl in H;
+        assert (depth s1 + depth s2 + depth s3 <=
+                  max (depth s1) (depth t1) + max (depth s2) (depth t2) +
+                  max (depth s3) (depth t3)) as H'
+          by (apply Nat.add_le_mono; try apply Nat.add_le_mono; trivial);
+        try apply Nat.le_trans with (max (depth s1) (depth t1) + max (depth s2) (depth t2) +
+                                 max (depth s3) (depth t3)); trivial ). apply p_s3_s1.
+      + (* t1 <: t2 <: t3 *) intros; apply IHn with (unbindT y t2) k0 k k1;
+        try (rewrite depth_unbindT; repeat rewrite depth_unbindT);
+        assert (depth t1 <= max (depth s1) (depth t1)) 
+          as Hdep1 by apply Nat.le_max_r;
+        assert (depth t2 <= max (depth s2) (depth t2)) 
+          as Hdep2 by apply Nat.le_max_r;
+        assert (depth t3 <= max (depth s3) (depth t3)) 
+          as Hdep3 by apply Nat.le_max_r;
+        repeat rewrite <- plus_n_Sm in H; simpl in H; 
+        apply Nat.lt_le_incl in H; apply Nat.lt_le_incl in H;
+        assert (depth t1 + depth t2 + depth t3 <=
+                  max (depth s1) (depth t1) + max (depth s2) (depth t2) +
+                  max (depth s3) (depth t3)) as H'
+          by (apply Nat.add_le_mono; try apply Nat.add_le_mono; trivial);
+        try apply Nat.le_trans with (max (depth s1) (depth t1) + max (depth s2) (depth t2) +
+                                 max (depth s3) (depth t3)); 
+        try apply WFEBind with k_x1; try apply H24;
+        try apply H12;
+        try apply lem_narrow_subtype_top with s2 k_x1 k_x0 k0 k;
+        try apply H7; 
+        try apply lem_narrow_wf_top with s2; try apply H21;
+        try apply lem_narrow_wf_top with s1; try apply H18;
+        repeat (apply not_elem_union_elim in H9; destruct H9);
+        try apply wfenv_unique; trivial. 
+    * (* -ANY- SWitn *)  apply SWitn with v_x0; trivial;
+      apply IHn with t' k k' k''; try rewrite depth_tsubBV;
+      subst t''; simpl in H;
+      repeat rewrite <- plus_n_Sm in H; rewrite <- Nat.succ_le_mono in H;
+      assert (depth t'1 <= max (depth t_x0) (depth t'1)) 
+        as Hdep by apply Nat.le_max_r;
+      apply Nat.add_le_mono_l with (depth t'1) (max (depth t_x0) (depth t'1))
+                                  (depth t + depth t') in Hdep;
+      try apply Nat.le_trans with (depth t + depth t' + max (depth t_x0) 
+                                                        (depth t'1));
+      trivial; inversion H3;
+      try inversion H17; try apply WFKind;
+      pose proof (fresh_var_not_elem nms g) as Hy;
+      set (y := fresh_var nms g) in Hy; destruct Hy as [Hy Hy'];
+      try rewrite lem_tsubFV_unbindT with y v_x0 t'1;
+      try apply lem_subst_wf_top with t_x0;
+      try apply lem_typing_hasftype;
+      pose proof (lem_free_bound_in_env g (TExists t_x0 t'1) k'' y H3 Hy') as Hfr;
+      simpl in Hfr; destruct Hfr as [Hfr _];
+      apply not_elem_union_elim in Hfr as [_ Hfr]; 
+      try apply wfenv_unique; simpl; intuition.
+    * (* SWitn SBind *) apply IHn with (tsubBV v_x t'0) k k' k'';
+      try rewrite depth_tsubBV; subst t'; simpl in H;
+      rewrite <- plus_n_Sm in H; simpl in H; rewrite <- Nat.succ_le_mono in H;
+      assert (depth t'0 <= max (depth t_x) (depth t'0)) 
+        as Hdep by apply Nat.le_max_r;
+      apply Nat.add_le_mono_l with (depth t'0) (max (depth t_x) (depth t'0))
+                                  (depth t) in Hdep;
+      apply Nat.add_le_mono_r with (depth t + depth t'0) 
+                                  (depth t + max (depth t_x) (depth t'0))
+                                  (depth t'') in Hdep;
+      try apply Nat.le_trans with (depth t + max (depth t_x) (depth t'0) + depth t'');
+      trivial; inversion H2; try inversion H11;
+      injection H15 as Htx0 Ht1; subst t_x0; subst t1;
+      pose proof (fresh_var_not_elem (union nms nms0) g) as Hy;
+      set (y := fresh_var (union nms nms0) g) in Hy; destruct Hy as [Hy Hy'];
+      apply not_elem_union_elim in Hy; destruct Hy;  
+      rewrite lem_tsubFV_unbindT with y v_x t'0;
+      try apply lem_subst_wf_top with t_x; try apply WFKind;
+      try apply H21; try apply H25;
+      assert (t'' = tsubFV y v_x t'') as Ht''
+        by (symmetry; apply lem_subFV_notin; 
+            try apply lem_free_bound_in_env with g k''; trivial);
+      try rewrite Ht''; try apply lem_subst_subtype_top with t_x k' k'';
+      try apply H13; try apply H21;
+      try (apply lem_weaken_wf_top; assumption);
+      pose proof (lem_free_bound_in_env g (TExists t_x t'0) k' y H2 Hy') as Hfr;
+      simpl in Hfr; destruct Hfr as [Hfr _];
+      apply not_elem_union_elim in Hfr as [_ Hfr]; 
+      try apply wfenv_unique; try apply lem_typing_hasftype;
+      destruct k'; try apply WFKind; try apply H25; trivial.
+    * (* SPoly SPoly *) subst t'; injection H12 as Hk0 Ht0;
+      subst k0; subst t0; subst t; subst t'';
+      inversion H1; try inversion H8;
+      inversion H2; try inversion H16;
+      inversion H3; try inversion H22;
+      apply SPoly 
+        with (union (union (union (union (union nms nms0) nms1) nms2) nms3) (binds g));
+      intros; repeat (apply not_elem_union_elim in H28; destruct H28);
+      apply IHn with (unbind_tvT a t2) k k' k''; subst k k' k'';
+      try (rewrite depth_unbind_tvT; repeat rewrite depth_unbind_tvT);
+      simpl in H; repeat rewrite <- plus_n_Sm in H;
+      rewrite <- Nat.succ_le_mono in H;
+      apply Nat.lt_le_incl in H; simpl in H; apply Nat.lt_le_incl in H; try apply H;
+      try apply WFEBindT;
+      try apply H6; try apply H10;
+      destruct k_t;  try (apply H14 || (apply WFKind; apply H14));
+      destruct k_t0; try (apply H20 || (apply WFKind; apply H20));
+      destruct k_t1; try (apply H26 || (apply WFKind; apply H26));
+      try apply wfenv_unique; trivial.
+    * (* SList SList *) subst t'; injection H14; intros; subst t t'' t0 p0.
+      apply SList with (union (union nms nms0) (binds g));
+      try apply IHn with t2 Star Star Star; intros;
+      try (apply lem_wflist_wftype with p1 k;   apply H1);
+      try (apply lem_wflist_wftype with p2 k';  apply H2);
+      try (apply lem_wflist_wftype with p3 k''; apply H3);
+      try apply ITrans with (unbindP y p2); try apply H7;
+      try assert (ECons y (TList t1 PEmpty) g 
+                    = concatE (ECons y (TList t1 PEmpty) g) Empty)
+          as Henv by (reflexivity); try rewrite Henv;
+      try apply INarrow with (TList t2 PEmpty) Star Star; 
+      try apply SList with nms; intros; try apply IRefl;
+      try apply WFList with Star;
+      try (apply lem_wflist_wftype with p1 k;   apply H1);
+      try (apply lem_wflist_wftype with p2 k';  apply H2);     
+      simpl in H; repeat rewrite <- plus_n_Sm in H;
+      rewrite <- Nat.succ_le_mono in H;
+      apply Nat.lt_le_incl in H; simpl in H; apply Nat.lt_le_incl in H; try apply H;
+      try apply not_elem_union_elim in H9; try destruct H9;
+      try apply not_elem_union_elim in H9; try destruct H9;
+      try apply intersect_empty_r;
+      try apply wfenv_unique; try apply WFEEmpty; simpl; auto.
+  Qed.
+  
+Lemma lem_sub_trans : forall (g:env) (t t' t'':type) (k k' k'':kind),
+    WFEnv g -> WFtype g t k -> WFtype g t' k' -> WFtype g t'' k'' 
+            -> Subtype g t t' -> Subtype g t' t'' 
+            -> Subtype g t t''.
+Proof. intros; 
+  apply lem_sub_trans' with (depth t + depth t' + depth t'') t' k k' k'';
+  trivial. Qed.
