coq-SystemRF-3.0/SystemRF/PrimitivesDeltaTyping.v
@@ -1,0 +1,545 @@
+Require Import SystemRF.BasicDefinitions.
+Require Import SystemRF.Names.
+Require Import SystemRF.LocalClosure.
+Require Import SystemRF.Semantics.
+Require Import SystemRF.SystemFWellFormedness.
+Require Import SystemRF.SystemFTyping.
+Require Import SystemRF.BasicPropsSubstitution.
+Require Import SystemRF.BasicPropsEnvironments.
+Require Import SystemRF.WellFormedness.
+Require Import SystemRF.PrimitivesFTyping.
+Require Import SystemRF.PrimitivesWFType.
+Require Import SystemRF.BasicPropsWellFormedness.
+Require Import SystemRF.SystemFLemmasWellFormedness.
+Require Import SystemRF.Typing.
+Require Import SystemRF.LemmasWeakenWF.
+Require Import SystemRF.LemmasWellFormedness.
+Require Import SystemRF.SubstitutionLemmaWF.
+Require Import SystemRF.LemmasTyping.
+Require Import SystemRF.LemmasSubtyping.
+Require Import SystemRF.LemmasExactness. 
+Require Import SystemRF.SubstitutionLemmaTyp.
+Require Import SystemRF.SubstitutionLemmaTypTV.
+Require Import SystemRF.LemmasTransitive.
+Require Import SystemRF.LemmasInversion.
+
+Require Import ZArith.
+
+(* -- Lemma. Typing of \delta(c,v) and \delta_T(c,t) *)
+Lemma lem_delta_ty'c : forall (c:prim) (v:expr),
+    ~ isPoly c -> ~ isMeasure c -> isValue v -> Hastype Empty v (intype c)
+               -> exists e, Some e = delta' c v /\ Hastype Empty e (tsubBV v (ty' c)).
+Proof. intros c v np nm val p_v_inc; destruct c eqn:C;
+  simpl in np; simpl in nm; try contradiction;
+  apply lem_typing_hasftype in p_v_inc as Hv; try apply WFEEmpty;
+  simpl in Hv;
+  try apply (lem_bool_values v val) in Hv;
+  try apply (lem_int_values v val) in Hv;
+  destruct v eqn:V; simpl in Hv; try contradiction;
+  assert (isCompat c v) as pf by (rewrite C; rewrite V; constructor);
+  assert (forall m:Z, isCompat Leq (Ic m)) as pfL by constructor;
+  assert (forall m:Z, isCompat Eq  (Ic m)) as pfE by constructor;
+  assert (isCompatT Eql (TRefn TBool PEmpty)) as pfB by (apply isCptT_EqlB; trivial);
+  assert (isCompatT Eql (TRefn TInt  PEmpty)) as pfZ by (apply isCptT_EqlZ; trivial);
+  assert (forall m:Z, delta Leq (Ic m) (pfL m) = Prim (Leqn m)) as delL
+      by (intro m; pose proof (delta_delta' Leq (Ic m) (pfL m)) as D; 
+          simpl in D; injection D; trivial);
+  assert (forall m:Z, delta Eq  (Ic m) (pfE m) = Prim (Eqn m))  as delE
+      by (intro m; pose proof (delta_delta' Eq  (Ic m) (pfE m)) as D; 
+          simpl in D; injection D; trivial);
+  assert ( Prim Eqv = deltaT Eql (TRefn TBool PEmpty) pfB ) as delTB
+    by (pose proof (deltaT_deltaT' Eql (TRefn TBool PEmpty) pfB) as D;
+        simpl in D; injection D; trivial );
+  assert ( Prim Eq  = deltaT Eql (TRefn TInt PEmpty) pfZ ) as delTZ
+    by (pose proof (deltaT_deltaT' Eql (TRefn TInt PEmpty) pfZ) as D;
+        simpl in D; injection D; trivial );        
+  try destruct b; unfold tsubBV; simpl;
+  ( match goal with
+    | [ |- exists _, Some _ = Some ?term /\ _ ] 
+           => assert (delta c v pf = term) as del
+                by ( pose proof (delta_delta' c v pf) as D; 
+                     subst c; subst v; simpl in D; injection D; trivial ) ; 
+              exists term
+    end )
+          ; split ; try reflexivity 
+          ; try apply TAbs with Base empty 
+          ; try apply WFBase; trivial; intros       (* remove? *)
+          ; unfold unbind; unfold unbindT; simpl ;  (* remove? *) 
+  ( try match goal with
+    | [ |- Hastype _ (FV ?yy) _ ] =>
+            apply TSub 
+              with (TRefn TBool (PCons (App (App (Prim Eqv) (FV yy)) (BV 0)) 
+                                       PEmpty)) Base
+          ; try apply TSub with (self (TRefn TBool PEmpty) (FV yy)  Base) Base
+          ; try apply SBase with (singleton y); intros; unfold unbindP ;
+          try ( apply IEvals; rewrite delTB; apply lem_step_evals; 
+                apply EApp1; apply EApp1; apply EPrimT; trivial ) ;
+          try ( apply IEvals2;
+                apply AddStep 
+                  with (App (App (Prim Eqv) (App (delta c v pf) (FV y))) (FV y0));
+                subst c; subst v;
+                try apply EApp1; try apply EApp2; 
+                  try apply EApp1; try apply EPrim; try rewrite del; 
+                try apply lem_step_evals; try apply EApp1; 
+                  try apply EApp2; try apply EAppAbs; intuition ) ;
+          try apply TVar
+    | [ |- Hastype (ECons _ _ _) (Bc ?bb) _ ] =>
+            apply TSub 
+              with (TRefn TBool (PCons (App (App (Prim Eqv) (Bc bb)) (BV 0)) 
+                                       PEmpty)) Base
+          ; try apply TSub with (self (TRefn TBool PEmpty)    (Bc bb)     Base) Base 
+          ; try apply SBase with (singleton y); intros; unfold unbindP; 
+          try ( apply IEvals; rewrite delTB; apply lem_step_evals; 
+                apply EApp1; apply EApp1; apply EPrimT; trivial ) ;
+          try ( apply IEvals2;
+                apply AddStep 
+                  with (App (App (Prim Eqv) (App (delta c v pf) (FV y))) (FV y0));
+                subst c; subst v;
+                try apply EApp1; try apply EApp2; 
+                  try apply EApp1; try apply EPrim; try rewrite del; 
+                try apply lem_step_evals; try apply EApp1; 
+                  try apply EApp2; try apply EAppAbs; intuition ) ;
+          try apply TBC
+    | [ |- Hastype Empty (Bc ?bb) _ ] =>
+            apply TSub 
+              with (TRefn TBool (PCons (App (App (Prim Eqv) (Bc bb)) (BV 0)) 
+                                       PEmpty)) Base
+          ; try apply TSub with (self (TRefn TBool PEmpty)    (Bc bb)     Base) Base
+          ; try apply SBase with empty; intros; unfold unbindP
+          ; try ( apply IEvals; rewrite delTB; apply lem_step_evals; 
+                  apply EApp1; apply EApp1; apply EPrimT; trivial ) 
+          ; try ( apply IEvals2; rewrite <- del; 
+                  ( match goal with
+                    | [ |- EvalsTo (App (App _ (App _ (Ic _))) _) _] 
+                            => try apply AddStep with (App (App (Prim Eqv) (App (Prim c) v)) (FV y))
+                    | [ |- _ ] => trivial
+                    end
+                  ) ; subst c; subst v;
+                  try apply lem_step_evals; apply EApp1; apply EApp2; try apply EApp1; 
+                  try (apply EPrim || (rewrite <- delL; try apply EPrim)
+                                   || (rewrite <- delE; try apply EPrim)); 
+                  intuition ) 
+          ; try apply TBC
+    | [ |- Hastype _ (Prim ?c') _ ] =>
+            apply TSub with (ty c') Star; try apply SFunc with empty; unfold intype;
+          try apply lem_sub_refl with Base; intros;
+          try apply SBase with (singleton y); intros; unfold unbindP; 
+          try apply IRefl;
+          try ( apply IEvals2; apply lem_step_evals; apply EApp1; apply EApp2;
+                try apply EApp1; try rewrite <- del; subst c; subst v; 
+                try apply EPrim; intuition );
+          try apply TPrm; 
+          try apply WFFunc with Base Base empty; intros
+    | [ |- Hastype Empty (Ic ?nn) _ ] =>
+          apply TSub 
+              with (TRefn TInt (PCons (App (App (Prim Eq) (Ic nn)) (BV 0)) 
+                                       PEmpty)) Base
+          ; try apply TSub with (self (TRefn TInt PEmpty)    (Ic nn)     Base) Base
+          ; try apply SBase with empty; intros; unfold unbindP
+          ; try ( apply IEvals; rewrite delTZ; apply lem_step_evals; 
+                  apply EApp1; apply EApp1; apply EPrimT; trivial ) 
+          ; try ( apply IEvals2; rewrite <- del; simpl;
+                  apply lem_step_evals; apply EApp1; apply EApp2;
+                  subst c; subst v; try apply EPrim; constructor )
+          ; try apply TIC
+    end )  
+          ; try constructor ; intuition
+          ; try (apply WFRefn with (singleton y); try apply WFBase) 
+          ; try apply WFRefn with empty
+          ; try apply WFBase; intros; unfold unbindP; simpl
+          ; try apply PFTCons; try apply PFTEmp
+          ; try match goal with
+            | [ |- HasFtype (FCons _ (FTBasic TBool) _) _ _ ]
+                => try apply FTApp with (FTBasic TBool)
+            | [ |- HasFtype (FCons _ (FTBasic TInt) _) _ _ ]
+                => try apply FTApp with (FTBasic TInt)
+            end
+          ; try match goal with
+            | [ |- HasFtype (FCons _ (FTBasic TBool) _) _ _ ]
+                => try apply FTApp with (FTBasic TBool)
+            | [ |- HasFtype (FCons _ (FTBasic TInt) _) _ _ ]
+                => try apply FTApp with (FTBasic TInt)
+            end
+          ; try ( apply FTApp with (FTBasic TInt); 
+                  try apply FTApp with (FTBasic TInt); 
+                  apply FTPrm || apply FTIC || apply FTVar) 
+          ; try apply FTApp with (FTBasic TBool) 
+          ; try apply FTApp with (FTBasic TBool)
+          ; try apply FTPrm; try apply FTVar
+          ; try apply FTBC ; try apply FTIC
+          ; try discriminate ; simpl ; intuition.
+  Qed.
+
+Lemma lem_deltaT_ty'c : forall (c:prim) (t:type),
+    isPoly c -> noExists t -> WFtype Empty t Base
+               -> exists e, Some e = deltaT' c t /\ 
+                            Hastype Empty e (tsubBTV t (TFunc (intype c) (ty' c))).
+Proof. intros c t ispo noex p_emp_t; destruct c eqn:C;
+  simpl in ispo; try contradiction;
+  apply lem_erase_wftype in p_emp_t as Ht;
+  apply lem_base_types in Ht; destruct t eqn:T; try destruct b eqn:B;
+  simpl in Ht; try contradiction;
+  unfold deltaT'; unfold erase;
+  ( match goal with
+    | [ |- exists _, Some _ = Some ?term /\ _ ] => exists term
+    end ) 
+          ; split ; unfold tsubBTV; simpl
+          ; try ( match goal with 
+                  | [ |- Hastype _ (Prim ?c) _ ] => apply TSub with (ty c) Star
+                  end ) 
+          ; try apply TPrm
+          ; try apply WFFunc with Base Star empty; intros
+          ; try apply WFFunc with Base Base (singleton y) ; intros ; fold openP_at 
+          ; try assert (openP_at (0 + 1) y ps = ps) as Hps
+              by ( apply lem_wftype_islct in p_emp_t as lct;  
+                   unfold isLCT in lct; simpl in lct;         
+                   apply lem_open_at_lc_at with 0; assumption )
+          ; try assert (openP_at (0 + 1 + 1 + 1) y ps = ps) as Hps3
+              by ( apply lem_wftype_islct in p_emp_t as lct;  
+                   unfold isLCT in lct; simpl in lct;         
+                   apply lem_open_at_lc_at with 0; 
+                   apply lem_islc_at_weaken with 1 0; auto with * )              
+          ; try rewrite Hps ; try rewrite Hps3; try reflexivity 
+
+          ; try apply WFRefn with (names_add y0 (singleton y))
+          ; try apply WFBase; fold openP_at; fold open_at 
+          ; try apply lem_weaken_wf_top; intros
+          ; destruct (Nat.eqb (0 + 1 + 1) 0) eqn:E0
+          ; destruct (Nat.eqb (0 + 1 + 1) 1) eqn:E1
+          ; destruct (Nat.eqb (0 + 1 + 1) 2) eqn:E2
+          ; try (simpl in E0; discriminate E0)
+          ; try (simpl in E1; discriminate E1)
+          ; try (simpl in E2; discriminate E2)
+          ; unfold unbindP; simpl; try assumption 
+          ; try assert (openP_at 2 y0 ps = ps) as Hps2
+              by ( apply lem_wftype_islct in p_emp_t as lct;  
+                   unfold isLCT in lct; simpl in lct;         
+                   apply lem_open_at_lc_at with 0; 
+                   apply lem_islc_at_weaken with 1 0; auto with *  )
+          ; try assert (openP_at 1 y1 ps = ps) as Hps1
+              by ( apply lem_wftype_islct in p_emp_t as lct;  
+                   unfold isLCT in lct; simpl in lct;         
+                   apply lem_open_at_lc_at with 0; assumption  ) 
+          ; try rewrite Hps2; try rewrite Hps1
+
+          ; try apply PFTCons; try apply PFTEmp; try discriminate 
+          ; try apply FTApp with (FTBasic TBool) 
+          ; try apply FTApp with (FTBasic TBool) 
+          ; try ( apply FTApp with (FTBasic TBool); apply FTPrm || apply FTVar; 
+                  simpl; intuition ) 
+          ; try apply FTApp with (FTBasic b)
+          ; try apply FTApp with (FTBasic b) 
+          ; try assert ( FTFunc (FTBasic b) (FTFunc (FTBasic b) (FTBasic TBool)) 
+                          = ftsubBV (erase (TRefn b ps)) 
+                                    (FTFunc (FTBasic (BTV 0)) 
+                                            (FTFunc (FTBasic (BTV 0)) (FTBasic TBool))))
+              as H' by reflexivity
+          ; try rewrite H' ; try rewrite B 
+          ; try apply FTAppT with Base
+          ; try apply FTVar ; try apply FTPrm 
+          ; try apply WFFTBasic
+
+          ; try pose proof (lem_free_subset_binds Empty (TRefn TBool ps) Base p_emp_t) as Hf
+          ; try pose proof (lem_free_subset_binds Empty (TRefn TInt  ps) Base p_emp_t) as Hf
+          ; simpl; simpl in Hf; destruct Hf as [Hfv Hftv]
+          ; try (apply Hftv || apply subset_trans with empty)
+          ; try apply subset_empty_l
+          ; try apply lem_wftype_islct with Empty Base
+          ; try discriminate
+          ; simpl ; try rewrite B ; auto with *
+
+          ; apply SFunc with empty 
+          ; try apply SBase with empty; intros; try apply IFaith
+          ; intros; unfold unbindT; simpl 
+          ; apply SFunc with (singleton y)
+          ; try apply SBase with (singleton y); intros; try apply IFaith
+          ; intros; unfold unbindT; simpl
+          ; apply SBase with (names_add y0 (singleton y)) 
+          ; intros; unfold unbindP; simpl 
+          ; apply IEvals2
+          ; try set (qs := (openP_at 1 y1 (openP_at 2 y0 (openP_at 3 y ps)))) 
+          ; ( match goal with 
+              | [ |- EvalsTo (App (App (Prim Eqv)
+                                  (App (App (AppT (Prim ?c) (TRefn ?b _)) _) _)) _) 
+                             (App (App (Prim Eqv) (App (App (Prim ?c') _) _)) _) ] 
+                        => assert (isCompatT c (TRefn b qs)) 
+                              as pf by (constructor; trivial) ;
+                           assert ( Prim c' = deltaT c (TRefn b qs) pf ) as delT
+                              by (pose proof (deltaT_deltaT' c (TRefn b qs) pf) as D;
+                                  simpl in D; injection D; trivial ) 
+              end )
+          ; apply lem_step_evals
+          ; apply EApp1; apply EApp2; try apply EApp1; try apply EApp1
+          ; trivial ; try constructor
+          ; try rewrite delT ; try apply EPrimT ; trivial.
+  Qed.
+
+Lemma lem_deltaM_ty'c : forall (c:prim) (t:type) (v:expr),
+    isMeasure c -> noExists t -> isMono t -> WFtype Empty t Star
+                -> isValue v -> Hastype Empty v (tsubBTV t (intype c))
+                -> exists e, Some e = deltaM' c v /\
+                             Hastype Empty e (tsubBV v (tsubBTV t (ty' c))). 
+Proof. intros c t v isMeas noex mono p_emp_t Hval; 
+  induction Hval; intro p_v;
+  destruct c eqn:C; simpl in isMeas; try contradiction;
+  unfold tsubBTV in p_v; simpl in p_v;
+  rewrite lem_push_empty in p_v;
+  try apply lem_typing_hasftype in p_v as p_v'; try simpl in p_v';
+  try apply lemma_list_values in p_v' as Hv;
+  try constructor; try apply WFEEmpty; try assumption;
+  try simpl in Hv; try contradiction;
+  
+  assert (isCompatT Eql (TRefn TInt  PEmpty)) as pfZ by (apply isCptT_EqlZ; trivial);
+  assert ( Prim Eq  = deltaT Eql (TRefn TInt PEmpty) pfZ ) as delTZ
+    by (pose proof (deltaT_deltaT' Eql (TRefn TInt PEmpty) pfZ) as D;
+        simpl in D; injection D; trivial ).
+  - (* v = Nil *) 
+    assert (isCompatM c Nil) as pf by (rewrite C; constructor).
+    assert (deltaM c Nil pf = (Ic 0)) as del
+                by ( pose proof (deltaM_deltaM' c Nil pf) as D; 
+                     subst c; simpl in D; injection D; trivial ).
+    simpl; exists (Ic 0); split;
+    try reflexivity; unfold tsubBTV; unfold tsubBV;
+    simpl; rewrite lem_push_empty; try apply noex;
+    try apply lem_wftype_islct in p_emp_t as Hlct. 
+    pose proof lem_subBV_at_lc_at as [_ [H _]].
+    rewrite H with t 1 Nil 0 0; 
+    pose proof lem_open_at_lc_at as [_ [H1 _]]; intuition.
+
+    apply TSub 
+        with (TRefn TInt (PCons (App (App (Prim Eq) (Ic 0)) (BV 0)) 
+                                PEmpty)) Base
+    ; try apply TSub with (self (TRefn TInt PEmpty) (Ic 0) Base) Base
+    ; try apply SBase with empty; intros; unfold unbindP; simpl
+    ; try ( apply IEvals; rewrite delTZ; apply lem_step_evals; 
+            apply EApp1; apply EApp1; apply EPrimT; trivial ) 
+    ; try ( rewrite H1 with t 0 0 y; try apply Hlct;
+            apply IEvals2; apply lem_step_evals;
+            apply EApp1; apply EApp2; try rewrite <- del; 
+            subst c; try apply EPrimM; constructor )
+    ; try apply TIC
+    ; try apply WFRefn with empty
+    ; try apply WFBase
+    ; intros; unfold unbindP; simpl
+    ; try apply PFTCons ; try apply PFTEmp
+    ; try rewrite H1 with t 0 0 y
+    ; try apply FTApp with (FTBasic TInt)
+    ; try apply FTApp with (FTBasic TInt)
+    ; try apply FTApp with (FTList (erase t))
+    ; assert (FTFunc (FTList (erase t)) (FTBasic TInt)
+            = ftsubBV (erase t) (FTFunc (FTList (FTBasic (BTV 0))) 
+                                        (FTBasic TInt)))
+        as Henv by reflexivity
+    ; try rewrite Henv ; try apply FTAppT with Star
+    ; try apply FTPrm ; try apply FTNil with Star
+    ; try apply FTVar ; try apply FTIC
+    ; try apply lem_weaken_wfft_top
+    ; assert (erase_env Empty = FEmpty)
+        as Henv2 by reflexivity; try rewrite <- Henv2
+    ; try apply lem_erase_wftype ; try apply p_emp_t
+    ; apply lem_free_subset_binds in p_emp_t as [Hfv Hftv]
+    ; simpl in Hfv ; simpl in Hftv
+    ; try apply subset_trans with empty
+    ; try apply subset_empty_l
+    ; try discriminate; simpl; auto.
+  - (* v = Cons *) simpl. (*inversion p_v.*)
+    pose proof TCons.
+
+
+    destruct IHHval2 as [n Hn];
+    unfold tsubBTV; simpl; rewrite lem_push_empty;
+    try apply noex.
+    (* Emp |- v2 : [t]{true} *)
+    destruct v2; simpl in Hv; try contradiction.
+
+    pose proof TNil.
+    pose proof TCons.
+
+    inversion p_v.
+
+
+
+
+
+
+
+
+
+  apply lemma_list_values with v (erase t) in Hval as Hv.
+  pose proof lemma_list_values.
+
+Lemma lem_prim_compat_in_tapp : forall (p:prim) (v:expr) (t:type),
+    isValue v -> Hastype Empty (App (Prim p) v) t -> isCompat' p v.
+Proof. intros p v t val p_pv_t; apply lem_prim_compat_in_ftapp with (erase t);
+  assert (erase_env Empty = FEmpty) by reflexivity; try rewrite <- H;
+  try apply lem_typing_hasftype; try apply WFEEmpty; assumption. Qed.
+  
+Lemma lem_prim_compatT_in_tappT : forall (c:prim) (t_a t:type),
+    noExists t_a -> Hastype Empty (AppT (Prim c) t_a) t -> isCompatT' c t_a.
+Proof. intros c t_a t noex p_cta_t; apply lem_prim_compatT_in_ftappt with (erase t);
+  assert (erase_env Empty = FEmpty) by reflexivity; try rewrite <- H;
+  try apply lem_typing_hasftype; try apply WFEEmpty; assumption. Qed.
+
+Lemma lem_invert_prim : forall (g:env) (pc:expr) (t:type),
+  Hastype g pc t -> (forall (c : prim) (s_x s' : type),
+    pc = Prim c -> WFEnv g -> Subtype g t (TFunc s_x s')
+                -> WFtype g (TFunc s_x s') Star
+                -> Subtype g (ty c) (TFunc s_x s')).
+Proof. apply ( Hastype_ind
+    ( fun (g:env) (pc:expr) (t:type) => forall (c : prim) (s_x s' : type),
+        pc = Prim c -> WFEnv g -> Subtype g t (TFunc s_x s')
+                -> WFtype g (TFunc s_x s') Star
+                -> Subtype g (ty c) (TFunc s_x s'))
+  ); try discriminate; intros.
+  - (* isTPrm *) injection H as C; subst c0; assumption.
+  - (* isTSub *) apply H0; try apply lem_sub_trans with t Star k Star;
+    try (apply lem_typing_wf with e; assumption); assumption.
+  Qed.
+  
+Lemma lem_delta_typ : forall (c:prim) (v:expr) (t_x t': type),
+    isValue v -> Hastype Empty (Prim c) (TFunc t_x t') -> Hastype Empty v t_x
+              -> exists e, Some e = delta' c v /\ Hastype Empty e (TExists t_x t').
+Proof. intros c v t_x t' val p_c_txt' p_v_tx. inversion p_c_txt';
+  assert (Hastype Empty (App (Prim c) v) (TExists t_x t')) as p_cv_txt'
+    by (apply TApp; assumption);
+  assert (isCompat c v) as pf 
+    by (apply compat_prop_set;
+        apply lem_prim_compat_in_tapp with (TExists t_x t'); assumption);
+  exists (delta c v pf); rewrite delta_delta'; split; try reflexivity.
+  - (* isTPrm *) assert (ty c = TFunc (intype c) (ty' c)) as Hty
+        by (destruct c; simpl in H2; try discriminate H2; simpl; reflexivity);
+    assert (~ isPoly c) as Hmono
+        by (destruct c; simpl in Hty; try discriminate Hty; intuition);
+    rewrite Hty in H2; injection H2 as Htx Ht'; subst t_x t';
+    apply TSub with (tsubBV v (ty' c)) Star;
+    (* Hastype Empty (delta c v pf) (tsubBV v (ty' c)) *)
+    pose proof (lem_delta_ty'c c v Hmono val p_v_tx); destruct H0; destruct H0;
+    rewrite <- delta_delta' with c v pf in H0; injection H0 as H0; 
+    subst x ; try apply H2;
+    (* Subtype Empty (tsubBV v (ty' c)) (TExists (intype c) (ty' c)) *)
+    try apply lem_witness_sub with Star; try apply WFEEmpty;
+    (* WFtype Empty (TExists (intype c) (ty' c)) Star *)
+    pose proof (lem_wf_ty' c Hmono); destruct H0 as [nms Hty'];
+    try apply WFExis with Base nms;
+    try apply lem_wf_intype; try apply Hty'; trivial.
+  - (* isTSub *) assert (Subtype Empty (ty c) (TFunc t_x t')) as p_tyc_txt'
+        by (apply lem_invert_prim with (Prim c) (TFunc t_x t'); 
+            try apply WFEEmpty; try apply lem_sub_refl with Star;
+            destruct k; try (apply H0 || (apply WFKind; apply H0)); trivial);
+    inversion p_tyc_txt'; try (destruct c; simpl in H5; discriminate H5);
+    assert (ty c = TFunc (intype c) (ty' c)) as Hty
+        by (destruct c; simpl in H5; try discriminate H5; simpl; reflexivity);
+    assert (~ isPoly c) as Hmono
+        by (destruct c; simpl in Hty; try discriminate Hty; intuition);
+    apply TSub with (tsubBV v (ty' c)) Star; subst g0 s2 t2;
+    rewrite Hty in H5; injection H5 as Hs1 Ht1; subst s1 t1;
+    assert (Hastype Empty v (intype c)) as p_v_in
+      by (apply TSub with t_x Base; try apply lem_wf_intype; assumption);
+    (* Hastype Empty (delta c v pf) (tsubBV v (ty' c)) *)
+    pose proof (lem_delta_ty'c c v Hmono val p_v_in) as H';
+    rewrite <- delta_delta' with c v pf in H';
+    destruct H' as [x H']; destruct H';
+    try rewrite <- delta_delta' with c v pf in H5; injection H5 as H5; 
+    subst x ; try apply H6;
+    (* Subtype Empty (tsubBV v (ty' c)) (TExists t_x t' *)
+    try apply lem_sub_trans with (TExists t_x (ty' c)) Star Star Star;
+    pose proof (lem_wf_ty' c Hmono); destruct H5 as [nms' Hty'];
+    pose proof (fresh_not_elem nms'); set (y := fresh nms') in H5;
+    try apply lem_witness_sub with Star;
+    try apply lem_subtype_in_exists with Star (union nms nms');
+    try (intros y0 Hy0; apply not_elem_union_elim in Hy0;
+         destruct Hy0; apply H10; assumption);    
+    try apply lem_wftype_islct with Empty Star;
+    try rewrite lem_tsubFV_unbindT with y v (ty' c);
+    try (destruct c; simpl; unfold not; intro ff; apply ff);
+    try apply lem_subst_wf_top with (intype c); try apply Hty';
+    try apply lem_witness_sub with Star;
+    (* WFtype Empty (TExists (intype c) (ty' c)) Star, etc *)
+    inversion H0; try inversion H7;
+    try apply WFExis with Star (union nms' nms0);
+    try intros y0 Hy0; try apply not_elem_union_elim in Hy0;
+    try destruct Hy0; destruct k0;
+    try (apply H14 || (apply WFKind; apply H14));
+    try apply lem_narrow_wf_top with (intype c); try apply Hty';
+    try apply lem_typing_wf with v;
+    try apply lem_typing_hasftype;
+    try apply WFEEmpty;   simpl; intuition.
+  Qed.
+
+Lemma lem_invert_primT : forall (g:env) (pc:expr) (t:type),
+  Hastype g pc t -> (forall (c : prim) (k : kind) (s' : type),
+    pc = Prim c -> WFEnv g -> Subtype g t (TPoly k s')
+                -> WFtype g (TPoly k s') Star
+                -> Subtype g (ty c) (TPoly k s')).
+Proof. apply ( Hastype_ind
+  ( fun (g:env) (pc:expr) (t:type) => forall (c: prim) (k:kind) (s':type),
+        pc = Prim c -> WFEnv g -> Subtype g t (TPoly k s')
+                    -> WFtype g (TPoly k s') Star
+                    -> Subtype g (ty c) (TPoly k s'))
+  ); try discriminate; intros.
+  - (* isTPrm *) injection H as C; subst c0; assumption.
+  - (* isTSub *) apply H0; try apply lem_sub_trans with t Star k Star;
+    try (apply lem_typing_wf with e; assumption); assumption.
+  Qed.
+
+Lemma lem_tyeql_forallbase : forall (c:prim) (k:kind) (s:type),
+    Subtype Empty (ty c) (TPoly k s) -> k = Base.
+Proof. intros c k s p_tyc_ks; inversion p_tyc_ks;
+  destruct c; simpl in H; try discriminate H; 
+  injection H as Hk Hty'; subst k0; intuition. Qed.
+
+Lemma lem_deltaT_typ : forall (c:prim) (t:type) (k:kind) (s': type),
+    isMono t -> noExists t -> Hastype Empty (Prim c) (TPoly k s') 
+              -> WFtype Empty t k
+              -> exists e, Some e = deltaT' c t /\ Hastype Empty e (tsubBTV t s').
+Proof. intros c t k s' mono noex p_c_ks' p_emp_t. inversion p_c_ks';
+  assert (Hastype Empty (AppT (Prim c) t) (tsubBTV t s')) as p_ct_s't
+    by (apply TAppT with k; assumption);
+  assert (isCompatT c t) as pf 
+    by (apply compatT_prop_set;
+        apply lem_prim_compatT_in_tappT with (tsubBTV t s'); assumption);
+  exists (deltaT c t pf); rewrite <- deltaT_deltaT'; split; try reflexivity;
+  try assert (Subtype Empty (ty c) (TPoly k s')) as p_tyc_ks' (* if TSub *)
+        by (apply lem_invert_primT with (Prim c) (TPoly k s'); 
+            try apply WFEEmpty; try apply lem_sub_refl with Star;
+            destruct k0; try (apply H0 || (apply WFKind; apply H0)); trivial);
+  try inversion p_tyc_ks'; try (destruct c; simpl in H5; discriminate H5);
+  assert (ty c = TPoly Base (TFunc (intype c) (ty' c))) as Hty
+    by (destruct c; simpl in H2; try discriminate H2; 
+        try simpl in H5; try discriminate H5; simpl; reflexivity);
+  assert (isPoly c) as Hpoly
+    by (destruct c; simpl in Hty; try discriminate Hty; simpl; intuition);
+  rewrite Hty in H2 || rewrite Hty in H5; 
+  injection H2 as Hk Ht' || injection H5 as Hk Ht'.
+  - (* isTPrm *) subst s'; subst k;
+    pose proof (lem_deltaT_ty'c c t Hpoly noex p_emp_t); 
+    destruct H0 as [e H0]; destruct H0;
+    rewrite deltaT_deltaT' with c t pf in H0; injection H0 as H0; subst e; assumption.
+  - (* isTSub *) inversion H0; try inversion H5; 
+    pose proof (lem_wf_ty Empty c) as Htyc;
+    rewrite Hty in Htyc; inversion Htyc; try inversion H15.
+    subst k k0 k1 k2 k3 g0 g1 g2 t1 t2 t3 t4;
+    apply TSub with (tsubBTV t (TFunc  (intype c) (ty' c))) Star;
+    (* Hastype Empty (deltaT c t pf) (tsubBTV t (TFunc (intype c) (ty' c))) *)
+    pose proof (lem_deltaT_ty'c c t Hpoly noex p_emp_t) as H';
+    rewrite deltaT_deltaT' with c t pf in H';
+    destruct H' as [x H']; destruct H'; injection H5 as H5; 
+    subst x ; try apply H6;
+    (* WFtype Empty (tsubFTV a t (unbind_tvT a s')) Star *)
+    try apply lem_typing_wf with (AppT (Prim c) t); try apply p_ct_s't;
+    (* Subtype Empty (tsubBTV t (TFunc (intype c) (ty' c))) (tsubBTV t s') *)
+    pose proof (fresh_not_elem (union nms (union nms0 nms1))) as Ha; 
+    set (a := fresh (union nms (union nms0 nms1))) in Ha;
+    apply not_elem_union_elim in Ha; destruct Ha;
+    apply not_elem_union_elim in H7; destruct H7;
+    try rewrite lem_tsubFTV_unbind_tvT with a t (TFunc (intype c) (ty' c));
+    try rewrite lem_tsubFTV_unbind_tvT with a t s';
+    try apply lem_subst_tv_subtype_top with Base Star k_t; try apply H11;
+    assert (~ in_env a Empty) as Htriv by intuition;
+    pose proof (lem_free_bound_in_env Empty (TPoly Base s') Star a H0 Htriv) 
+      as Hfr; simpl in Hfr; destruct Hfr;
+      try (destruct c; simpl; unfold not; intro ff; apply ff);
+    try apply WFEEmpty; simpl; auto;
+    destruct k_t0; try apply H17; try apply WFKind; 
+    try apply H17; auto.
+  Qed.
