coq-SystemRF-3.0/compile.sh
@@ -65,22 +65,22 @@ echo "Checking SubstitutionLemmaTyp.v ..."
 coqc -R SystemRF SystemRF SystemRF/SubstitutionLemmaTyp.v
 echo "Checking SubstitutionLemmaTypTV.v ..."
 coqc -R SystemRF SystemRF SystemRF/SubstitutionLemmaTypTV.v
-#echo "Checking LemmasNarrowing.v ..."
-#coqc -R SystemRF SystemRF SystemRF/LemmasNarrowing.v
-#echo "Checking LemmasTransitive.v ..."
-#coqc -R SystemRF SystemRF SystemRF/LemmasTransitive.v
-#echo "Checking LemmasInversion.v ..."
-#coqc -R SystemRF SystemRF SystemRF/LemmasInversion.v
+echo "Checking LemmasNarrowing.v ..."
+coqc -R SystemRF SystemRF SystemRF/LemmasNarrowing.v
+echo "Checking LemmasTransitive.v ..."
+coqc -R SystemRF SystemRF SystemRF/LemmasTransitive.v
+echo "Checking LemmasInversion.v ..."
+coqc -R SystemRF SystemRF SystemRF/LemmasInversion.v
 #echo "Checking PrimitivesDeltaTyping.v ..."
 #coqc -R SystemRF SystemRF SystemRF/PrimitivesDeltaTyping.v
 #echo "Checking MainTheorems.v ..."
 #coqc -R SystemRF SystemRF SystemRF/MainTheorems.v
 
-#echo "Up next: Implement the Denotational Semantics Development"
-#echo "Checking ClosingSubstitutions.v ..."
-#coqc -Q SystemRF SystemRF -R Denotations Denotations Denotations/ClosingSubstitutions.v
-#echo "Checking Denotations.v ..."
-#coqc -Q SystemRF SystemRF -R Denotations Denotations Denotations/Denotations.v
+echo "Up next: Implement the Denotational Semantics Development"
+echo "Checking ClosingSubstitutions.v ..."
+coqc -Q SystemRF SystemRF -R Denotations Denotations Denotations/ClosingSubstitutions.v
+echo "Checking Denotations.v ..."
+coqc -Q SystemRF SystemRF -R Denotations Denotations Denotations/Denotations.v
 #echo "Checking PrimitivesSemantics.v ..."
 #coqc -Q SystemRF SystemRF -R Denotations Denotations Denotations/PrimitivesSemantics.v
 #echo "Checking BasicPropsCSubst.v ..."
